\section{Appendix}\label{sec-appendix}

\subsection{Proof of Theorem \ref{theo-regs}}\label{subsec-appendix-estimators}

We define the first-differenced regressors as follows.
\[ \Delta \mathbf{X}_{it} =\mathbf{H}_i(\mathcal{U}_{it}) - \mathbf{H}_i(\mathcal{U}_{it-1}) := \Delta \mathbf{H}_i(\mathcal{U}_{it}). \]
Similarly, 
\[\Delta \varepsilon_{it} = \varepsilon_{it} - \varepsilon_{it-1} = G_i(\mathcal{J}_{it}) - G_i(\mathcal{J}_{it-1}) = \Delta G_i(\mathcal{J}_{it}).
\]
 
With these assumptions we can prove the following propositions.
\begin{prop}\label{prop-reg-1}
Under Assumptions \ref{C-reg1} and \ref{C-reg3}, $|| \Delta \mathbf{H}_i(\mathcal{U}_{it})||_4 < \infty$.
\end{prop}

\begin{proof}[\textnormal{\textbf{Proof of Proposition \ref{prop-reg-1}}}]
By Assumption \ref{C-reg3},
\[
 || \Delta \mathbf{H}_i(\mathcal{U}_{it})||_4 \leq  ||\mathbf{H}_i(\mathcal{U}_{it})||_4 +  || \mathbf{H}_i(\mathcal{U}_{it-1})||_4 < \infty.
\]
\end{proof} 

\begin{prop}\label{prop-reg-2}
Under Assumption \ref{C-reg4}, $\Delta \mathbf{X}_{it}$ (elementwise) and $\Delta \varepsilon_{it}$ are uncorrelated for each $t\in \{1, \ldots, T\}$.
\end{prop}

\begin{proof}[\textnormal{\textbf{Proof of Proposition \ref{prop-reg-2}}}]
By Assumption \ref{C-reg4},
\begin{align*}
\ex [\Delta \mathbf{X}_{it}\Delta \varepsilon_{it}] &= \ex \big[(\mathbf{X}_{it} - \mathbf{X}_{it-1}) (\varepsilon_{it} - \varepsilon_{it-1})\big] =\\
=&\ex[\mathbf{X}_{it}  \varepsilon_{it}] - \ex[\mathbf{X}_{it-1}  \varepsilon_{it}]- \ex[\mathbf{X}_{it}  \varepsilon_{it-1}] + \ex[\mathbf{X}_{it-1}  \varepsilon_{it-1}] =\\
=& \ex[\mathbf{X}_{it}]\ex[  \varepsilon_{it}] - \ex[\mathbf{X}_{it-1}]\ex[  \varepsilon_{it}]- \ex[\mathbf{X}_{it}]\ex[  \varepsilon_{it-1}] + \ex[\mathbf{X}_{it-1}]\ex[  \varepsilon_{it-1}] =\\
=& \big( \ex[\mathbf{X}_{it}] - \ex[\mathbf{X}_{it-1}]\big)\big(\ex[  \varepsilon_{it}]  - \ex[\varepsilon_{it-1}]\big) = \ex [\Delta \mathbf{X}_{it}]\ex[\Delta \varepsilon_{it}]
\end{align*}
\end{proof} 


\begin{prop}\label{prop-reg-3}
Define 
\[ \Delta \mathbf{U}_i(\mathcal{I}_{i, t}) := \Delta \mathbf{H}_i(\mathcal{U}_{it}) \Delta G_i(\mathcal{J}_{it}).
\]
Under Assumptions \ref{C-err2} - \ref{C-err3}, \ref{C-reg5} - \ref{C-reg6}, we have that $\sum_{s=0}^\infty \delta_2(\Delta \mathbf{U}_i, s) < \infty$.
\end{prop}

\begin{proof}[\textnormal{\textbf{Proof of Proposition \ref{prop-reg-3}}}]
Note the following
\begin{align*}
 &\delta_2(\Delta \mathbf{U}_i, t) = || \Delta\mathbf{U}_i(\mathcal{I}_{i, t}) - \Delta \mathbf{U}_i(\mathcal{I}_{i,t}^\prime) ||_2 =\\
 &= || \Delta \mathbf{H}_i(\mathcal{U}_{it}) \Delta G_i(\mathcal{J}_{it}) -  \Delta \mathbf{H}_i(\mathcal{U}_{it}^\prime) \Delta G_i(\mathcal{J}_{it}^\prime) ||_2 =\\
 & = ||\big(\mathbf{H}_i(\mathcal{U}_{it}) - \mathbf{H}_i(\mathcal{U}_{it-1})\big)\big(G_i(\mathcal{J}_{it}) - G_i(\mathcal{J}_{it-1})\big) - \big(\mathbf{H}_i(\mathcal{U}_{it}^\prime) - \mathbf{H}_i(\mathcal{U}_{it-1}^\prime)\big)\big(G_i(\mathcal{J}_{it}^\prime) - G_i(\mathcal{J}_{it-1}^\prime)\big)||_2 =\\
 &= ||\mathbf{H}_i(\mathcal{U}_{it})G_i(\mathcal{J}_{it}) - \mathbf{H}_i(\mathcal{U}_{it-1})G_i(\mathcal{J}_{it}) - \mathbf{H}_i(\mathcal{U}_{it})G_i(\mathcal{J}_{it-1})  + \mathbf{H}_i(\mathcal{U}_{it-1})G_i(\mathcal{J}_{it-1}) - \\
 &\quad - \mathbf{H}_i(\mathcal{U}_{it}^\prime)G_i(\mathcal{J}_{it}^\prime) + \mathbf{H}_i(\mathcal{U}_{it-1}^\prime)G_i(\mathcal{J}_{it}^\prime) + \mathbf{H}_i(\mathcal{U}_{it}^\prime)G_i(\mathcal{J}_{it-1}^\prime)  - \mathbf{H}_i(\mathcal{U}_{it-1}^\prime)G_i(\mathcal{J}_{it-1}^\prime) ||_2\leq \\
 &\leq ||\mathbf{H}_i(\mathcal{U}_{it})G_i(\mathcal{J}_{it}) - \mathbf{H}_i(\mathcal{U}_{it}^\prime)G_i(\mathcal{J}_{it}^\prime) ||_2 + ||\mathbf{H}_i(\mathcal{U}_{it-1})G_i(\mathcal{J}_{it-1}) -  \mathbf{H}_i(\mathcal{U}_{it-1}^\prime)G_i(\mathcal{J}_{it-1}^\prime)||_2 + \\
 &\quad + ||\mathbf{H}_i(\mathcal{U}_{it-1})G_i(\mathcal{J}_{it}) -\mathbf{H}_i(\mathcal{U}_{it-1}^\prime)G_i(\mathcal{J}_{it}^\prime)    ||_2
 + ||\mathbf{H}_i(\mathcal{U}_{it})G_i(\mathcal{J}_{it-1}) -  \mathbf{H}_i(\mathcal{U}_{it}^\prime)G_i(\mathcal{J}_{it-1}^\prime) ||_2 = \\
 & = \delta_2(\mathbf{U}_i, t) + \delta_2(\mathbf{U}_i, t-1)  +\\
 &\quad + ||\mathbf{H}_i(\mathcal{U}_{it-1})G_i(\mathcal{J}_{it}) - \mathbf{H}_i(\mathcal{U}_{it-1}^\prime)G_i(\mathcal{J}_{it}) + \mathbf{H}_i(\mathcal{U}_{it-1}^\prime)G_i(\mathcal{J}_{it}) - \mathbf{H}_i(\mathcal{U}_{it-1}^\prime)G_i(\mathcal{J}_{it}^\prime)    ||_2+\\
 &\quad + ||\mathbf{H}_i(\mathcal{U}_{it})G_i(\mathcal{J}_{it-1}) -\mathbf{H}_i(\mathcal{U}_{it}^\prime)G_i(\mathcal{J}_{it-1})+ \mathbf{H}_i(\mathcal{U}_{it}^\prime)G_i(\mathcal{J}_{it-1})-  \mathbf{H}_i(\mathcal{U}_{it}^\prime)G_i(\mathcal{J}_{it-1}^\prime) ||_2 \leq\\
  &\leq \delta_2(\mathbf{U}_i, t) + \delta_2(\mathbf{U}_i, t-1)  + \\
  &\quad +||\big(\mathbf{H}_i(\mathcal{U}_{it-1}) - \mathbf{H}_i(\mathcal{U}_{it-1}^\prime)\big) G_i(\mathcal{J}_{it})||_2 +  ||\mathbf{H}_i(\mathcal{U}_{it-1}^\prime)\big(G_i(\mathcal{J}_{it}) - G_i(\mathcal{J}_{it}^\prime)\big)    ||_2+\\
 &\quad + ||\big(\mathbf{H}_i(\mathcal{U}_{it}) -\mathbf{H}_i(\mathcal{U}_{it}^\prime)\big)G_i(\mathcal{J}_{it-1})||_2 + ||\mathbf{H}_i(\mathcal{U}_{it}^\prime)\big(G_i(\mathcal{J}_{it-1}) -G_i(\mathcal{J}_{it-1}^\prime)\big) ||_2 \leq \\
 &\leq \delta_2(\mathbf{U}_i, t) + \delta_2(\mathbf{U}_i, t-1)  + \big(\delta_2(\mathbf{H}_i, t-1) +  \delta_2(\mathbf{H}_i, t)\big) ||G_i ||_2+ \big( \delta_2(G_i, t-1) +  \delta_2(G_i, t)\big)||\mathbf{H}_i ||_2  
\end{align*}

Here $\mathcal{U}_{it}^\prime  = (\ldots, u_{i(-1)}, u^\prime_{i0}, u_{i1}, \ldots, u_{it-1}, u_{it})$, $\mathcal{U}_{it-1}^\prime  = (\ldots, u_{i(-1)}, u^\prime_{i0}, u_{i1}, \ldots, u_{it-1})$, $\mathcal{J}_{it}^\prime  = (\ldots, \eta_{i(-1)}, \eta^\prime_{i0}, \eta_{i1}, \ldots, \eta_{it-1}, \eta_{it})$, $\mathcal{J}_{it-1}^\prime  = (\ldots, \eta_{i(-1)}, \eta^\prime_{i0}, \eta_{i1}, \ldots, \eta_{it-1})$ are coupled processes with $u_{i0}^\prime$ being an i.i.d. copy of $u_{i0}$ and $\eta_{i0}^\prime$ being an i.i.d. copy of $\eta_{i0}$.

This leads us to 
\begin{align*}
 &\sum_{s=0}^\infty \delta_2(\Delta \mathbf{U}_i, s) \leq \sum_{s=0}^\infty \delta_2(\mathbf{U}_i, s) + \sum_{s=1}^\infty\delta_2(\mathbf{U}_i, s-1)  +\\
 &\quad + \sum_{s=1}^\infty\big(\delta_2(\mathbf{H}_i, s-1) +  \delta_2(\mathbf{H}_i, s)\big) ||G_i ||_2 + \sum_{s=1}^\infty\big( \delta_2(G_i, s-1) +  \delta_2(G_i, s)\big)||\mathbf{H}_i ||_2 <\infty 
\end{align*}


\end{proof}


\begin{prop}\label{prop-reg-4}
Under Assumptions \ref{C-err1} - \ref{C-reg6},
\[ \Big| \frac{1}{\sqrt{T}}\sum_{t=1}^T \Delta \mathbf{X}_{it}\Delta \varepsilon_{it} \Big| = O_P(1).
\]
\end{prop}

\begin{proof}[\textnormal{\textbf{Proof of Proposition \ref{prop-reg-4}}}]
We need the following notation:
\begin{alignat*}{2}
&\mathcal{P}_{i,t}(\cdot) &&:= \ex[\cdot|\mathcal{I}_{i, t}] -\ex[\cdot|\mathcal{I}_{i, t-1}], \\
&\kappa_{i} && := \frac{1}{T}\sum_{t=1}^T  \Delta \mathbf{X}_{it}\Delta \varepsilon_{it}, \\
&\kappa_{i, s}^{\mathcal{P}} && := \frac{1}{T}\sum_{t=1}^T \mathcal{P}_{i, t-s}\big( \Delta \mathbf{X}_{it}\Delta \varepsilon_{it}\big).
\end{alignat*}
Then,
\begin{align*}
||\kappa_{i, s}^{\mathcal{P}}||^2 &= \Big|\Big| \frac{1}{T}\sum_{t=1}^T \mathcal{P}_{i, t-s}\big( \Delta \mathbf{X}_{it}\Delta \varepsilon_{it}\big) \Big|\Big|^2 \leq\\
&\leq \frac{1}{T^2} \sum_{t=1}^T \Big|\Big| \ex (\Delta \mathbf{X}_{it}\Delta \varepsilon_{it}|\mathcal{I}_{i, t-s}) -\ex (\Delta \mathbf{X}_{it}\Delta \varepsilon_{it}|\mathcal{I}_{i, t-s-1}) \Big|\Big|^2 =\\
&= \frac{1}{T^2} \sum_{t=1}^T \Big|\Big| \ex (\Delta \mathbf{X}_{it}\Delta \varepsilon_{it}|\mathcal{I}_{i, t-s}) -\ex (\Delta \mathbf{X}_{it, s}^\prime\Delta \varepsilon_{it, s}^\prime|\mathcal{I}_{i, t-s}) \Big|\Big|^2,
\end{align*}
where $\Delta \mathbf{X}_{it, s}^\prime\Delta \varepsilon_{it, s}^\prime$ denotes $\Delta \mathbf{X}_{it}\Delta \varepsilon_{it}$ with $\{\zeta_{i, t-s}\}$ replaced by its i.i.d. copy $\{\zeta_{i, t-s}^\prime\}$. In this case $\ex (\Delta \mathbf{X}_{it, s}^\prime\Delta \varepsilon_{it, s}^\prime|\mathcal{I}_{i, t-s -1}) = \ex (\Delta \mathbf{X}_{it, s}^\prime\Delta \varepsilon_{it, s}^\prime|\mathcal{I}_{i, t-s})$. Furthermore, by linearity of the expectation and Jensen's inequality, we have 
\begin{align*}
||\kappa_{i, s}^{\mathcal{P}}||^2 &\leq \frac{1}{T^2} \sum_{t=1}^T \Big|\Big| \ex (\Delta \mathbf{X}_{it}\Delta \varepsilon_{it}|\mathcal{I}_{i, t-s}) -\ex (\Delta \mathbf{X}_{it, s}^\prime\Delta \varepsilon_{it, s}^\prime|\mathcal{I}_{i, t-s}) \Big|\Big|^2 \leq \\
&\leq \frac{1}{T^2} \sum_{t=1}^T \Big|\Big| \Delta \mathbf{X}_{it}\Delta \varepsilon_{it} -\Delta \mathbf{X}_{it, s}^\prime\Delta \varepsilon_{it, s}^\prime\Big|\Big|^2 =\\
& = \frac{1}{T^2} \sum_{t=1}^T \Big|\Big| \Delta \mathbf{H}_i(\mathcal{U}_{it})  \Delta G_i(\mathcal{J}_{it}) - \Delta \mathbf{H}_i(\mathcal{U}_{it, s}^\prime)  \Delta G_i(\mathcal{J}_{it, s}^\prime)\Big|\Big|^2 =\\
& = \frac{1}{T^2} \sum_{t=1}^T \Big|\Big| \Delta \mathbf{U}_i(\mathcal{I}_{i,t})  - \Delta \mathbf{U}_i(\mathcal{I}_{i,t, s}^\prime) \Big|\Big|^2 \leq \frac{1}{T^2} \sum_{t=1}^T \delta_2^2(\Delta \mathbf{U}_i, s) = \frac{1}{T}\delta_2^2(\Delta \mathbf{U}_i, s)
\end{align*}
with $\mathcal{U}_{it, s}^\prime = (\ldots, u_{it-s-1}, u^\prime_{it-s}, u_{it-s+1}, \ldots, u_{it})$, $\mathcal{J}_{it, s}^\prime = (\ldots, \eta_{it-s-1}, \eta^\prime_{it-s}, \eta_{it-s+1}, \ldots, \eta_{it})$, $\zeta^\prime_{it} = (u_{it}^\prime, \eta_{it}^\prime)^\top$ and $\mathcal{I}_{i,t,s}^\prime =(\ldots, \zeta_{it-s-1}, \zeta^\prime_{it-s}, \zeta_{it-s+1}, \ldots, \zeta_{it})$.

Moreover,
\begin{align*}
\kappa_i - \ex \kappa_i &= \frac{1}{T}\sum_{t=1}^T \Delta \mathbf{X}_{it}\Delta \varepsilon_{it} - \ex \kappa_i = \frac{1}{T}\sum_{t=1}^T \ex ( \Delta \mathbf{X}_{it}\Delta \varepsilon_{it}|\mathcal{I}_{i,t}) - \ex \kappa_i =\\
&= \frac{1}{T}\sum_{t=1}^T \big( \ex ( \Delta \mathbf{X}_{it}\Delta \varepsilon_{it}|\mathcal{I}_{i,t} ) - \ex ( \mathbf{X}_{it}\Delta \varepsilon_{it}) \big) = \\
&= \frac{1}{T}\sum_{t=1}^T \sum_{s=0}^\infty \big( \ex ( \Delta \mathbf{X}_{it}\Delta \varepsilon_{it}|\mathcal{I}_{i,t-s} ) - \ex ( \Delta \mathbf{X}_{it}\Delta \varepsilon_{it}|\mathcal{I}_{i,t-s-1} )  \big) =\\
&= \frac{1}{T}\sum_{t=1}^T \sum_{s=0}^\infty \mathcal{P}_{i, t-s} (\Delta \mathbf{X}_{it}\Delta \varepsilon_{it}) = \sum_{s=0}^\infty \kappa_{i, s}^{\mathcal{P}}.
\end{align*}
Thus, by Proposition \ref{prop-reg-3},
\[ || \kappa_i - \ex \kappa_i || \leq \sum_{s=0}^\infty ||\kappa_{i, s}^{\mathcal{P}} || \leq \frac{1}{\sqrt{T}}\sum_{s=0}^\infty \delta_2(\Delta \mathbf{U}_i, s) = O\Big(\frac{1}{\sqrt{T}}\Big)
\]
Since $\ex \kappa_i = 0$ by Proposition \ref{prop-reg-2}, we conclude that
\[  \Big|\Big| \frac{1}{T}\sum_{t=1}^T  \Delta \mathbf{X}_{it}\Delta \varepsilon_{it} \Big|\Big| = O\Big(\frac{1}{\sqrt{T}}\Big).
\]
Therefore, the proposition follows.
\end{proof}



\begin{proof}[\textnormal{\textbf{Proof of Theorem \ref{theo-regs}}}]
Recall the differencing estimator $\widehat{\bm{\beta}}_i$:
\begin{align*}
\widehat{\bm{\beta}}_i &= \Big( \sum_{t=1}^T \Delta \mathbf{X}_{it} \Delta \mathbf{X}_{it}^\top \Big)^{-1} \sum_{t=1}^T \Delta \mathbf{X}_{it} \Delta Y_{it} =\\
& =  \Big( \sum_{t=1}^T \Delta \mathbf{X}_{it} \Delta \mathbf{X}_{it}^\top \Big)^{-1} \sum_{t=1}^T \Delta \mathbf{X}_{it} \bigg(\Delta \mathbf{X}_{it}^\top \bm{\beta}_i + \Delta \varepsilon_{it} + O\Big(\frac{1}{T}\Big) \bigg) =\\
&= \bm{\beta}_i +  \Big( \sum_{t=1}^T \Delta \mathbf{X}_{it} \Delta \mathbf{X}_{it}^\top \Big)^{-1} \sum_{t=1}^T \Delta \mathbf{X}_{it} \Delta \varepsilon_{it}
+  O\Big(\frac{1}{T}\Big) \Big( \sum_{t=1}^T \Delta \mathbf{X}_{it} \Delta \mathbf{X}_{it}^\top \Big)^{-1} \sum_{t=1}^T \Delta \mathbf{X}_{it}. 
\end{align*}
This leads to
\begin{align*}
\sqrt{T}( \widehat{\bm{\beta}}_i - \bm{\beta}_i) &=  \Big(\frac{1}{T} \sum_{t=1}^T \Delta \mathbf{X}_{it} \Delta \mathbf{X}_{it}^\top \Big)^{-1}\frac{1}{\sqrt{T}} \sum_{t=1}^T \Delta \mathbf{X}_{it} \Delta \varepsilon_{it} +\\
&+  O\Big(\frac{1}{\sqrt{T}}\Big) \Big( \frac{1}{T}\sum_{t=1}^T \Delta \mathbf{X}_{it} \Delta \mathbf{X}_{it}^\top \Big)^{-1} \frac{1}{T}\sum_{t=1}^T \Delta \mathbf{X}_{it}.
\end{align*}

Since 
\[\ex \Big[ \frac{1}{T}\sum_{t=1}^T \Delta H_{ij}(\mathcal{U}_{it})\Big] = 0\]
and 
\[\var \Big[ \frac{1}{T}\sum_{t=1}^T \Delta H_{ij}(\mathcal{U}_{it})\Big] \leq \frac{4}{T^2} \ex\big[H_{ij}^2(\mathcal{U}_{it})\big],\]
by Chebyshev's inequality we have that $\Big|\frac{1}{T}\sum_{t=1}^T \Delta H_{ij}(\mathcal{U}_{it})\Big| = O_P(1)$ for each $j\in\{1, \ldots, d\} $. And this in turn implies that
\begin{align}\label{proof-1}
\Big|\frac{1}{T}\sum_{t=1}^T \Delta \mathbf{H}_i (\mathcal{U}_{it}) \Big| = \Big| \frac{1}{T}\sum_{t=1}^T \Delta \mathbf{X}_{it}\Big| = O_P(1).
\end{align}


Similarly, by Proposition \ref{prop-reg-1} and Chebyshev's inequality, we have that for each $j, k\in\{1, \ldots, d\}$
\[  \Big|\frac{1}{T}\sum_{t=1}^T \Delta H_{ij}(\mathcal{U}_{it}) \Delta H_{ik}(\mathcal{U}_{it})\Big| = O_P(1),
\]
which leads to 
\begin{align}\label{proof-2}
\Big|\Big| \frac{1}{T}\sum_{t=1}^T \Delta \mathbf{H}_i (\mathcal{U}_{it})\Delta \mathbf{H}_i (\mathcal{U}_{it})^\top \Big|\Big| =\Big|\Big|\frac{1}{T}\sum_{t=1}^T\Delta \mathbf{X}_{it} \Delta \mathbf{X}_{it}^\top\Big|\Big| = O_P(1),
\end{align}
where $||A||$ with $A$ being a matrix is any matrix norm.

By Assumption \ref{C-reg2}, we know that $\ex [\Delta \mathbf{X}_{it} \Delta \mathbf{X}_{it}^\top] = \ex [\Delta \mathbf{X}_{i0} \Delta \mathbf{X}_{i0}^\top]$ is invertible, thus, 
\[\Bigg| \Bigg| \Big(\frac{1}{T}\sum_{t=1}^T\Delta \mathbf{X}_{it} \Delta \mathbf{X}_{it}^\top\Big)^{-1}\Bigg|\Bigg| = O_P(1).\]
By applying Proposition \ref{prop-reg-4}, \eqref{proof-1} and \eqref{proof-2}, the statement of the theorem follows.
\end{proof}

\subsection{Proof of Theorem \ref{theo-stat-equality-with-regs}}\label{subsec-appendix-stat-equaility}
